towards simplest completeness

MultiScalarMul_Abstract.ec
@@ -6,6 +6,16 @@ require import BitEncoding StdBigop Bigalg.
 (*---*) import Ring.IntID IntOrder BS2Int.
 (*---*) import Bigint BIA.
 
+(*  
+
+   P := (beta, x, y) 
+   1/ subset by "onCurve"
+   2/ equiv. rel by  
+ 
+       2.1/ non unique representation of "x" and "y"
+       2.2/ all variations of identity point
+
+*)
 
 (* unique representation of points on the curve *)
 type R.                  
@@ -36,6 +46,8 @@ axiom op_id (x : R) :  x +++ idR = x.
 axiom op_id' (x : R) : idR +++ x = x.
 axiom op_inv (a : R) :  a +++ -a = idR. 
 
+
+
 (* op iteration properties  *)
 axiom one_mul (a : R) : 1 *** a = a.
 axiom zero_mul (a : R) : 0 *** a = idR. 
@@ -57,36 +69,25 @@ axiom w_pos : 0 < w.
 axiom l_pos : 0 < l.
 axiom T_pos : 0 < T.
 
-op onCurve : F -> bool.
-op idF     : F -> bool.
-op embed   : F -> R.
+type Point.
+
+op onCurve : Point -> bool.
+op idF     : Point -> bool.
+op embed   : Point -> R.
+
+op perfect_table_pure  parg varg = 
+ (fun (j i : int) =>  (i *** (parg j)) +++ - varg).
 
 
-lemma nosmt addass (a b c : int) : a + (b + c) = (a + b) + c.    by smt(). qed.
-lemma nosmt muldist (a b c : int) : a * (b + c) = a * b + a * c. by smt(). qed.
-lemma nosmt eqsym ['a] (a b : 'a) : a = b => b = a.              by smt(). qed.
-
-lemma kik  (a b c d : R) :  a +++ b +++ (c +++ d) = a +++ c +++ (b +++ d). 
- by smt(op_assoc op_comm). qed.
-
-    
-lemma qiq : forall a, 0 <= a => forall (c : int), forall (b : R),
-   a *** b +++ c *** b = (a + c) *** b.
-apply natind. progress. smt.
-progress. rewrite nplus_dist. auto.
-have ->: (n + 1 + c) = ((n + c) + 1). smt().
-rewrite nplus_dist. 
-rewrite - H0. smt().    
-smt(op_comm op_assoc).
-qed.    
-
-    
+op r_distr : R distr.
 
 module type OutCalls = {
-  proc getU() : F
+  proc getU() : Point
+  proc getUniformU() : R
   proc getT(P : int -> R, v : R) : int -> int -> R
   proc getPT(P : int -> R, v : R) : bool * (int -> int -> R)
 }.
+
 
 module MultiScalarMul(O : OutCalls) = {
 
@@ -119,7 +120,8 @@ module MultiScalarMul(O : OutCalls) = {
       return vahe;
   }
 
-  
+
+
   proc doubleWtimes(p : R, w : int) = {
       var cnt;
       cnt <- 0;
@@ -130,6 +132,8 @@ module MultiScalarMul(O : OutCalls) = {
       return p;
   }
 
+
+  
 
   proc multiScalarMulR(P : int -> R, s : int -> int -> int, U : R) = {
     var v, acc, aux, result : R;
@@ -199,8 +203,11 @@ module MultiScalarMul(O : OutCalls) = {
     return (flag, result);
   }
 
+
+
+
   proc multiScalarMul(P : int -> R, s : int -> int -> int) = {
-    var u_cand : F;
+    var u_cand : Point;
     var flag : bool;
     var result;
 
@@ -212,14 +219,42 @@ module MultiScalarMul(O : OutCalls) = {
     } else{
       result <- (false, witness);    
     } 
+    return result;
+  }
 
+  proc multiScalarMul_Completeness(P : int -> R, s : int -> int -> int) = {
+    var u_cand : R;
+    var flag : bool;
+    var result;
 
+    u_cand <@ O.getUniformU();
+    result <@ multiScalarMulI(P,s,u_cand);
     return result;
   }
 
 
-}.
 
+  proc multiScalarMulII(P : int -> R, s : int -> int -> int, U : R, table : int -> int -> R ) = {
+    var acc, aux, result : R;
+
+    var ic, jc, cnt : int;
+    var flag, flagaux : bool;
+
+    flag    <- true;
+    flagaux <- true;
+    acc     <- l *** U;
+    ic      <- 0;
+    while (ic < T) {
+      acc <@ doubleWtimes(acc,w);
+      (flagaux, acc) <@ helperI(acc, table, ic, s);
+      flag <- flag && flagaux;
+      ic <- ic + 1;
+    }    
+    return (flag, acc);
+  }
+
+
+}.
 
 
 op multiScalarMulR  (s : int -> int -> int) (P : int -> R) 
@@ -231,371 +266,17 @@ op multiScalarMulR  (s : int -> int -> int) (P : int -> R)
           acc2 +++ (2 ^ (w * (T - 1 - i)) * s j i) *** (P j)) idR
         ) idR.
 
-section.
-
-declare module O <: OutCalls.
-declare module O_Partial <: OutCalls.
-
-declare axiom tableP parg varg : hoare [ O.getT : arg = (parg,varg)
-   ==> res = (fun (j i : int) =>  (i *** (parg j)) +++ - varg)  ].
-
-declare axiom tablePT parg varg : hoare [ O.getPT : arg = (parg,varg)
-   ==> res.`1 => (res.`2 = (fun (j i : int) =>  (i *** (parg j)) +++ - varg)  /\ (forall i j, res.`2 i j <> idR) )   ].
- 
-declare axiom getT_lossless : islossless O.getT.
-
-declare axiom tableP_ph parg varg : phoare [ O.getT : arg = (parg,varg)
-   ==> res = (fun (j i : int) =>  (i *** (parg j)) +++ - varg)  ] = 1%r.
-
-declare axiom tablePT_ph parg varg : phoare [ O.getPT : arg = (parg,varg)
-   ==> res.`1 => (res.`2 = (fun (j i : int) =>  (i *** (parg j)) +++ - varg)  /\ (forall i j, res.`2 i j <> idR) )   ] = 1%r.
 
 
-lemma helpereqs argacc argtable argic args  : 
- equiv [ MultiScalarMul(O).helperR ~ MultiScalarMul(O).helperI : 
-  arg{2} = (argacc, argtable, argic, args) /\ ={acc,table,ic,s}
-       /\ (forall i j, table{1} i j <> idR)
-     ==>  res{2}.`1 => (res{1} = res{2}.`2)].
-proc.
-while (={jc,acc,table,aux,s,ic} /\ (flag{2} => ={vahe})
- /\ (forall i j, table{1} i j <> idR)).
- wp. skip. progress.
-   have -> : vahe{1} = vahe{2}. smt().
-rewrite same_res. 
-  smt().
-  smt(). 
-  smt().
-  smt().
-wp. skip. progress. 
-qed.
-
-    
-   
-lemma helper_specR_ph argcc argT argic args  : 
- phoare [ MultiScalarMul(O).helperR : arg = (argcc, argT, argic,  args) 
-     ==>  res = argcc +++  iteri l (fun j acc => acc +++ argT j (args j argic)) idR ] = 1%r.
-proc.
-while (0 <= jc 
- /\ jc <= l 
- /\ (acc, table, ic,  s) = (argcc, argT, argic, args) 
- /\ vahe = acc +++   iteri jc (fun j acc => acc +++ argT j (args j argic)) idR) (l - jc).
-move => z.
-wp. skip. progress. smt(). smt(). rewrite iteriS. smt().
-   simplify.
-smt(op_assoc).
-smt().   
-   wp. skip. progress. smt(l_pos). 
-rewrite iteri0. auto.
-smt(op_id).
-smt().
-smt().
-qed.   
-
-
-lemma helper_specR_total  : 
- phoare [ MultiScalarMul(O).helperR : true ==>  true ] = 1%r.
-proc*.
-exists*  acc, table, ic, s.
-elim*. move => accV tableV icV sV.        
-call (helper_specR_ph accV tableV icV sV).
-auto.
+lemma qiq : forall a, 0 <= a => forall (c : int), forall (b : R),
+   a *** b +++ c *** b = (a + c) *** b.
+apply natind. progress. smt.
+progress. rewrite nplus_dist. auto.
+have ->: (n + 1 + c) = ((n + c) + 1). smt().
+rewrite nplus_dist. 
+rewrite - H0. smt().    
+smt(op_comm op_assoc).
 qed.    
 
 
-lemma helper_specR argcc argT argic args  : 
- hoare [ MultiScalarMul(O).helperR : arg = (argcc, argT, argic,  args) 
-     ==>  res = argcc +++  iteri l (fun j acc => acc +++ argT j (args j argic)) idR ].
-conseq (helper_specR_ph argcc argT argic args).   
-progress.
-qed.   
 
-
-lemma iteriZ : forall (n : int), 0 <= n =>  forall (z : int) (f : int -> R), z *** (iteri n (fun i acc => acc +++ f i) idR)
-     = iteri n (fun i acc => acc +++ z *** (f i)) idR.
-apply intind.     
-progress. rewrite iteri0. auto. rewrite iteri0. auto. 
-apply mul_idr.
-progress.
-rewrite iteriS. auto.
-rewrite iteriS. auto.
-simplify.
-rewrite - H0.     
-apply mul_plus_distr. 
-qed.
-     
-lemma iteriZZ :  forall (n : int), 0 <= n => forall (z : R)  (f : int -> R),
-   (iteri n (fun i acc => acc +++ f i +++ z) idR)
-     = (iteri n (fun i acc => acc +++ f i) idR)
-        +++ (iteri n (fun i acc => acc +++ z) idR).
-apply intind. progress. rewrite iteri0. auto.
-rewrite iteri0. auto. rewrite iteri0. auto. rewrite op_id. auto.
-progress.
-rewrite iteriS. auto.
-rewrite iteriS. auto.
-rewrite iteriS. auto.
-simplify.
-rewrite H0. simplify.
-smt (op_assoc op_comm).
-qed.     
-
-
-lemma iteriZZZ  : forall (n : int), 0 <= n => forall (z : R),
-  (iteri n (fun i acc => acc +++ z) idR)
-     = n *** z.
-apply intind. progress. rewrite iteri0. auto. rewrite zero_mul. auto.
-progress.
-rewrite iteriS. auto. simplify.
-rewrite H0.
-rewrite nplus_dist. smt.
-qed.     
-
-
- 
-    
- 
-lemma nosmt mulsc : forall (a : int), 0 <= a => forall b r,  a *** (b *** r) = (a * b) *** r.
-apply intind.
-    progress.
-rewrite zero_mul. rewrite zero_mul. auto.
-progress.
-    rewrite nplus_dist. auto.
-have ->: (i + 1) * b = i * b + b. smt().
-rewrite H0.    
-rewrite nplus_dist. smt.
-qed.    
-
-
-lemma doublewtimes_spec_ph argP argw :
- phoare [ MultiScalarMul(O).doubleWtimes : arg = (argP, argw) /\
-   0 <= argw  ==>  res = (2 ^ argw) *** argP  ] = 1%r.
-proc. 
-   while (cnt <= w /\ 0 <= argw /\ 0 <= cnt /\ p = (2 ^ cnt) *** argP) (w - cnt).
-move => z.    
-   wp.
-   skip. progress. smt(). smt().
-   rewrite qiq. smt.
-   have ->: (2 ^ cnt{hr} + 2 ^ cnt{hr}) = (2 * 2 ^ cnt{hr} ).
-   smt(@Int).
-   congr.
-   rewrite exprS. auto. auto.
-   smt().
-   wp. skip. progress. smt. smt().
-   smt(@Int).
-qed.
-
-
-lemma doublewtimes_spec argP argw :
- hoare [ MultiScalarMul(O).doubleWtimes : arg = (argP, argw) /\
-   0 <= argw  ==>  res = (2 ^ argw) *** argP  ].
-conseq (doublewtimes_spec_ph argP argw).   
-qed.   
-
-
-lemma multiscalarR_spec argP args argU : 
- hoare [ MultiScalarMul(O).multiScalarMulR : 
-  arg = (argP, args, argU) 
-     ==>  res = (multiScalarMulR  args argP)  ].
-proc. wp.
-while (0 <= ic
- /\ (2 ^ w - 1) *** U = v
- /\ table = (fun (j i : int) =>  (i *** (P j)) +++ - v)
- /\ ic <= T
- /\ acc = ((iteri ic
-            (fun i acc1 => acc1 +++
-              (iteri l
-                 (fun j acc2 => acc2 +++ (2 ^ (w * (ic - 1 - i)) * s j i) *** (P j)) idR)
-                 ) idR)) +++ l *** U).
-wp.
-ecall (helper_specR acc table ic s). simplify.
-wp.
-ecall (doublewtimes_spec acc w). skip. progress. smt(w_pos).
-smt(). smt().
-   rewrite mul_plus_distr.
-rewrite iteriZ.           smt().
-simplify.
-have -> : iteri ic{hr}
-  (fun (i : int) (acc0 : R) =>
-     acc0 +++
-     2 ^ w ***
-     iteri l
-       (fun (j : int) (acc2 : R) =>
-          acc2 +++ 2 ^ (w * (ic{hr} - 1 - i)) * s{hr} j i *** P{hr} j) idR)
-  idR
-     = iteri ic{hr}
-  (fun (i : int) (acc0 : R) =>
-     acc0 +++
-     iteri l
-       (fun (j : int) (acc2 : R) =>
-          acc2 +++ 2 ^ (w * (ic{hr}  - i )) * s{hr} j i *** P{hr} j) idR)
-  idR.
-apply eq_iteri.
-progress.
-rewrite iteriZ. smt(l_pos). congr.
-     apply eq_iteri. move => j acc.
-     progress. congr.
-      have ->: 2 ^ w *** (2 ^ (w * (ic{hr} - 1 - i)) * s{hr} j i *** P{hr} j)
-                = 2 ^ w * 2 ^ (w * (ic{hr} - 1 - i)) * s{hr} j i *** P{hr} j .
-  rewrite mulsc. smt. smt().
-        rewrite - exprD_nneg. smt(w_pos). smt(w_pos). smt().
-pose v := (2 ^ w - 1) *** U{hr}.
-have -> : iteri l
-  (fun (j : int) (acc0 : R) => acc0 +++ (s{hr} j ic{hr} *** P{hr} j +++ -v))
-  idR = iteri l
-  (fun (j : int) (acc0 : R) => acc0 +++ (s{hr} j ic{hr} *** P{hr} j)) idR +++
-     iteri l (fun (j : int) (acc0 : R) => acc0 +++ -v) idR.
-rewrite - iteriZZ. simplify.
-smt(l_pos). apply eq_iteri.  progress. smt.
-simplify.
-rewrite  iteriZZZ.
-simplify. smt(l_pos).
-rewrite kik .
-have ->: (2 ^ w *** (l *** U{hr}) +++ l *** -v) = l *** U{hr}.
-    rewrite /v.
-  rewrite  mulsc. smt.
-  have -> : l *** - (2 ^ w - 1) *** U{hr}
-    = (l * - (2 ^ w - 1)) *** U{hr}. rewrite  nmul_mul.  rewrite neg_mul. auto.
-   rewrite - nplus_dist. congr. smt().
-
-rewrite iteriS.
-smt(). simplify.
-have ->: 2 ^ 0 = 1. smt(@Int).
-smt().
-wp.
-ecall (tableP P v). wp. skip. progress. smt(T_pos).
-rewrite iteri0. auto. smt.
-rewrite /multiScalarMulInt.
-have -> : ic0 = T. smt().
-simplify.
-  have ->: iteri T
-  (fun (i : int) (acc1 : R) =>
-     acc1 +++
-     iteri l
-       (fun (j : int) (acc2 : R) =>
-          acc2 +++ 2 ^ (w * (T - 1 - i)) * s{hr} j i *** P{hr} j) idR) idR +++
-l *** U{hr} +++ - l *** U{hr}
-       = iteri T
-  (fun (i : int) (acc1 : R) =>
-     acc1 +++
-     iteri l
-       (fun (j : int) (acc2 : R) =>
-          acc2 +++ 2 ^ (w * (T - 1 - i)) * s{hr} j i *** P{hr} j) idR) idR +++
-  (l *** U{hr} +++ - l *** U{hr} ).
-smt(op_assoc).
-rewrite op_inv.
-  rewrite op_id.
-  rewrite /multiScalarMulR.
-auto.
-qed.
-
-
-lemma multiscalarR_spec_ph argP args argU : 
- phoare [ MultiScalarMul(O).multiScalarMulR : 
-  arg = (argP, args, argU) 
-     ==>  res = (multiScalarMulR  args argP)  ] = 1%r.
-phoare split ! 1%r 0%r. auto.
-   proc. wp.
-while true (T - ic). progress.
-wp.
-exists* acc, table, ic, s.
-elim*. move => accV tableV icV sV.
-call helper_specR_total.   
-call (_: arg = (accV, Top.w) ==> true).
-proc*. call (doublewtimes_spec_ph accV Top.w).
-skip. progress. smt(w_pos). skip.
-progress.
-smt().
-wp. call (_:true). apply getT_lossless. 
-wp. skip. progress. smt().
-hoare. simplify.   
-apply multiscalarR_spec.
-qed.
-
-lemma multieqs argP args argU  :
- equiv [ MultiScalarMul(O).multiScalarMulR 
-        ~ MultiScalarMul(O).multiScalarMulI :
-  arg{2} = (argP, args, argU) /\ ={P,s,U} /\ ={glob O}
-     ==>  res{2}.`1 => (res{1} = res{2}.`2)].
-proc.
-wp.
-while ((flag{2} => ={table,acc,U,s} /\ (forall i j, table{2} i j <> idR)) /\ (flag{2} => flagaux{2}) /\ ={ic}  ).
-wp.
-inline MultiScalarMul(O).helperR.
-inline MultiScalarMul(O).helperI.
-wp.
-while ((flag{2} /\ flag0{2} => ={vahe, acc0,table0,aux0,s0,ic0} /\ (forall i j, table0{2} i j <> idR)) /\ ={jc0}).
- wp. skip. progress.
-   have -> : vahe{1} = vahe{2}. smt().
-rewrite same_res.
-  smt().
-  smt().
-  smt().
-  smt().
-     smt().
-     smt().
-     smt().
-     smt().
-     smt().
-     smt().
-wp.
-inline MultiScalarMul(O).doubleWtimes.
-wp.
-   while ((flag{2} => ={p}) /\ ={w,cnt0}). wp. skip. progress.
-   smt(). wp. skip. progress.
-smt(). smt(). smt(). smt(). smt(). smt().
-   smt(). smt().  smt(). smt(). smt().
-wp. 
-
-ecall {1} (tableP_ph P{1} v{1} ).
-ecall {2} (tablePT_ph P{2} v{2}).    
-
-wp. skip. progress. smt(). smt().
-have -> :     acc_L = acc_R. smt(). auto.
-qed.
-
-lemma multiscalarI_spec_ph argP args  argU : 
- phoare [ MultiScalarMul(O).multiScalarMulI : 
-  arg = (argP, args, argU) 
-     ==>  res.`1 => res.`2 = (multiScalarMulR  args argP)  ] = 1%r.
-proof.
-bypr.
-progress.
-have ih: 1%r = Pr[MultiScalarMul(O).multiScalarMulR(P{m}, s{m}, U{m}) @ &m 
-  : res = multiScalarMulR args argP].
-byphoare (_: arg = (argP, args, argU) ==> _).
-conseq (multiscalarR_spec_ph argP args argU). smt(). auto.
-have : Pr[MultiScalarMul(O).multiScalarMulI(P{m}, s{m}, U{m}) @ &m :
-   res.`1 => res.`2 = multiScalarMulR args argP] >=
-Pr[MultiScalarMul(O).multiScalarMulR(P{m}, s{m}, U{m}) @ &m :
-   res = multiScalarMulR args argP].
-byequiv (_: _ ==> res{2}.`1 => res{2}.`2 = res{1} ).
-proc*.
-ecall (multieqs argP args argU).
-skip. progress. smt(). smt(). smt(). smt().
-auto.
-smt().
-smt.
-qed.
-
-lemma multiscalarI_spec_h argP args  argU : 
- hoare [ MultiScalarMul(O).multiScalarMulI : 
-  arg = (argP, args, argU) 
-     ==>  res.`1 => res.`2 = (multiScalarMulR  args argP)  ] .
-conseq (multiscalarI_spec_ph argP args argU).
-qed.   
-
-
-lemma multiscalar_spec_h argP args : 
- hoare [ MultiScalarMul(O).multiScalarMul : 
-  arg = (argP, args) 
-     ==>  res.`1 => res.`2 = (multiScalarMulR  args argP)  ] .
-proc.
-seq 1 : #pre.
-call (_: true). auto.
-sp. if.
-  ecall (multiscalarI_spec_h P s (embed u_cand)).
-   skip. progress.
-wp. skip.
-smt().
-qed.   
-
-end section.
