MultiScalarMul_Abstract_Completeness.ec
@@ -1,0 +1,278 @@
+
+require import AllCore IntDiv CoreMap List.
+
+require import AllCore Int IntDiv List StdOrder Bool.
+require import BitEncoding StdBigop Bigalg.
+(*---*) import Ring.IntID IntOrder BS2Int.
+(*---*) import Bigint BIA.
+
+
+require import MultiScalarMul_Abstract.
+
+module NestedLoops = {
+
+
+
+  proc doubleWtimes(p : R, w : int) = {
+      var cnt;
+      cnt <- 0;
+      while (cnt < w) {
+        p <- p +++ p;
+        cnt <- cnt + 1;
+      }
+      return p;
+  }
+
+
+  proc helperI(acc : R, table : int -> int-> R, ic : int, s : int -> int -> int) =    {
+      var jc, aux, vahe, flag;
+    
+      aux <- witness;
+      flag <- true;
+      jc <- 0;
+      vahe <- acc;
+      while (jc < l) {
+        aux <- table jc (s jc ic);
+        flag <- flag && (xof vahe) <> (xof aux);
+        flag <- flag && (vahe <> idR);
+        vahe <- (vahe %%% aux);
+
+        jc <- jc + 1;
+      }
+      return (flag, vahe);
+  }
+
+
+  proc multiScalarMulII(P : int -> R, s : int -> int -> int, U : R, table : int -> int -> R ) = {
+    var acc, aux, result : R;
+
+    var ic, jc, cnt : int;
+    var flag, flagaux : bool;
+
+    flag    <- true;
+    flagaux <- true;
+    acc     <- l *** U;
+    ic      <- 0;
+    while (ic < T) {
+      acc <@ doubleWtimes(acc,w);
+      (flagaux, acc) <@ helperI(acc, table, ic, s);
+      flag <- flag && flagaux;
+      ic <- ic + 1;
+    }    
+    return (flag, acc);
+  }
+
+
+  proc multiScalarMul_Completeness_I(P : int -> R, s : int -> int -> int) = {
+    var u_cand : R;
+    var flag : bool;
+    var result, table;
+
+    u_cand <$ r_distr;
+    table  <- perfect_table_pure P ((2 ^ w - 1) *** u_cand) ; 
+    result <@ multiScalarMulII(P, s, u_cand, table);
+    return result;
+  }
+
+
+  proc multiScalarMul_Completeness_I_fun(P : int -> R, s : int -> int -> int) = {
+    var u_cand : R;
+    var flag : bool;
+    var result, table;
+
+    u_cand <$ r_distr;
+    table  <- perfect_table_pure P ((2 ^ w - 1) *** u_cand) ; 
+    result <- multiScalarMulII_pure T l table s (l *** u_cand) w;
+    return result;
+  }
+
+}.
+
+op predicate (x : R) (r : R) = xof x <> xof r && x <> idR.
+
+op helperI_pure (l : int) (argT : int -> int -> R)
+  (args : int -> int -> int) (argic : int) (argcc : R) 
+    = (iteri l (fun j (acc : bool * R) 
+        => (acc.`1 /\ predicate acc.`2 (argT j (args j argic)) , acc.`2 %%% argT j              (args j argic))) (true, argcc)).
+
+  
+op multiScalarMulII_pure (T l : int) (argT : int -> int -> R)
+  (args : int -> int -> int) (argu : R) (argw : int)
+    = (iteri T (fun i (acc : bool * R) 
+        => let r = helperI_pure l argT args i ((2 ^ argw) *** acc.`2) in (acc.`1 /\ r.`1, r.`2)) (true, argu)).
+
+
+lemma helperI_specR_ph argcc argT argic args  :
+ phoare [ NestedLoops.helperI : arg = (argcc, argT, argic,  args)
+     ==>  res = helperI_pure l argT args argic argcc ] = 1%r.
+proc.
+while (0 <= jc 
+ /\ jc <= l 
+ /\ flag = (iteri jc (fun j (acc : bool * R) => (acc.`1 /\ predicate acc.`2 (argT j (args j argic)) , acc.`2 %%% argT j (args j argic))) (true, argcc)).`1
+ /\ (acc, table, ic,  s) = (argcc, argT, argic, args) 
+ /\ vahe =  (iteri jc (fun j (acc : bool * R) => (acc.`1 /\ predicate acc.`2 (argT j (args j argic)) , acc.`2 %%% argT j (args j argic))) (true, argcc)).`2) (l - jc).
+move => z.
+wp. skip. progress. smt(). smt(). rewrite iteriS. smt().
+   simplify.
+   rewrite /predicate. 
+pose xxx := (iteri jc{hr}
+     (fun (j : int) (acc0 : bool * R) =>
+        (acc0.`1 /\
+         xof acc0.`2 <> xof (table{hr} j (s{hr} j ic{hr})) && acc0.`2 <> idR,
+         acc0.`2 %%% table{hr} j (s{hr} j ic{hr}))) (true, acc{hr})).
+
+pose yyy := (iteri jc{hr}
+       (fun (j : int) (acc0 : R) => acc0 %%% table{hr} j (s{hr} j ic{hr}))
+       acc{hr}).     smt().
+rewrite iteriS. smt().
+smt(op_assoc).
+smt().   
+   wp. skip. progress. smt(l_pos). 
+rewrite iteri0. auto. auto.
+rewrite iteri0. auto. auto.
+smt().   
+smt().
+qed.  
+
+
+
+lemma helperI_specR_h argcc argT argic args  :
+ hoare [ NestedLoops.helperI : arg = (argcc, argT, argic,  args)
+     ==>  res = helperI_pure l argT args argic argcc ].
+conseq (helperI_specR_ph argcc argT argic args).
+qed.   
+
+lemma doublewtimes_spec_ph argP argw :
+ phoare [ NestedLoops.doubleWtimes : arg = (argP, argw) /\
+   0 <= argw  ==>  res = (2 ^ argw) *** argP  ] = 1%r.
+proc. 
+   while (cnt <= w /\ 0 <= argw /\ 0 <= cnt /\ p = (2 ^ cnt) *** argP) (w - cnt).
+move => z.    
+   wp.
+   skip. progress. smt(). smt().
+   rewrite qiq. smt.
+   have ->: (2 ^ cnt{hr} + 2 ^ cnt{hr}) = (2 * 2 ^ cnt{hr} ).
+   smt(@Int).
+   congr.
+   rewrite exprS. auto. auto.
+   smt().
+   wp. skip. progress. smt. smt().
+   smt(@Int).
+qed.
+
+
+lemma doublewtimes_spec argP argw :
+ hoare [ NestedLoops.doubleWtimes : arg = (argP, argw) /\
+   0 <= argw  ==>  res = (2 ^ argw) *** argP  ].
+conseq (doublewtimes_spec_ph argP argw).   
+qed.   
+
+
+lemma multm_spec_h argP args argU argtable :
+ hoare [ NestedLoops.multiScalarMulII : arg = (argP, args, argU, argtable)   
+  ==>  res = multiScalarMulII_pure T l argtable args (l *** argU) w   ] .
+proc. 
+while (
+  0 <= ic 
+  /\ ic <= T
+  /\ (U, table, s) = (argU, argtable, args) 
+  /\ (flag , acc) = multiScalarMulII_pure ic l argtable args (l *** argU) w
+ ) .
+wp.
+ecall (helperI_specR_h acc argtable ic args).
+ecall (doublewtimes_spec acc w). 
+skip.
+progress. smt(w_pos).
+smt(). smt().
+rewrite /multiScalarMulII_pure.
+rewrite iteriS. smt().
+smt().
+wp. skip. progress. smt(T_pos).   
+rewrite /multiScalarMulII_pure. rewrite iteri0.
+auto. auto. 
+have -> : T = ic0. smt(T_pos).
+rewrite - H2.
+ smt().
+qed. 
+
+lemma multm_spec_ph argP args argU argtable :
+ phoare [ NestedLoops.multiScalarMulII : arg = (argP, args, argU, argtable)   
+  ==>  res = multiScalarMulII_pure T l argtable args (l *** argU) w   ]  = 1%r.
+phoare split ! 1%r 0%r. auto.
+   proc. wp.
+while (table = argtable /\ s = args) (T - ic). progress.
+wp.
+exists* acc, table, ic, s.
+elim*. move => accV tableV icV sV.
+call (helperI_specR_ph (2 ^ w *** accV) argtable icV args).
+call (doublewtimes_spec_ph accV MultiScalarMul_Abstract.w).
+skip.  progress. smt(w_pos).  smt().
+wp. progress.
+auto. smt(). hoare.
+apply multm_spec_h. 
+qed.
+
+
+lemma compl_I_equiv : 
+ equiv [ NestedLoops.multiScalarMul_Completeness_I_fun ~
+         NestedLoops.multiScalarMul_Completeness_I 
+     : ={arg} ==> ={res} ].
+proc.
+seq 2 2 : (#pre /\ ={u_cand, table}). wp. rnd. skip. progress.
+exists* P{2}, s{2}, u_cand{2}, table{2}. elim*. move => PV sV u_candV tableV.  
+call {2} (multm_spec_ph PV sV (u_candV) tableV).
+wp. skip. progress.
+qed.
+
+
+op p : real.
+print mu.
+ 
+(* mu r_distr *)
+(*  (fun (r : R) => (f r i acc).`1) <= p *)
+
+
+axiom iteri_ub ['a 'b] (g : 'a -> 'b) (f : 'a -> int -> 'b -> (bool * 'b)) (a_distr : 'a distr) (N : int) (p : real)  :
+
+  (forall i acc, mu a_distr
+    (fun (r : 'a) => (f r i acc).`1) <= p)
+
+  => 
+  mu a_distr 
+   (fun (x : 'a) => 
+      (iteri N (fun j (acc : bool * 'b) 
+        => 
+   let r = f x j acc.`2 in(acc.`1 /\ r.`1, r.`2)) (true,  g x)).`1  ) <= N%r * p.
+
+
+
+lemma completeness_I argP args :
+  phoare [ NestedLoops.multiScalarMul_Completeness_I_fun :
+      arg = (argP , args) ==> res.`1 ] <= (T%r * (l%r * p)).
+proc.
+wp. rnd. skip. progress. 
+rewrite /multiScalarMulII_pure.
+
+
+pose f := fun a i b => 
+  (helperI_pure l (perfect_table_pure P{hr} ((2 ^ w - 1) *** a))
+                s{hr} i (2 ^ w *** b)).
+
+
+apply  (iteri_ub (fun (x : R) => l *** x) f  r_distr T   ).  
+
+ move => i acc.
+rewrite /f. rewrite /helperI_pure.   
+
+pose h := fun  a j b
+    =>  ((predicate b
+               (perfect_table_pure P{hr} ((2 ^ w - 1) *** a) j (s{hr} j i)))
+        ,   
+   b %%%
+            perfect_table_pure P{hr} ((2 ^ w - 1) *** a) j (s{hr} j i)  ).
+
+apply  (iteri_ub (fun (x : R) => 2 ^ w *** acc) h  r_distr l  p).  
+progress.
+rewrite /h. simplify.           
+rewrite /perfect_table_pure. simplify.
+rewrite /predicate.            
